Updates

generic/Zeta.Generic.Global.fst
@@ -5,3 +5,21 @@ let lemma_prefix_verifiable #vspec (gl: verifiable_log vspec) (i:nat{i <= S.leng
           [SMTPat (SA.prefix gl i)]
   = admit()
 
+let add_sseq (#vspec:_) (gl: verifiable_log vspec)
+  : ss:sseq (ms_hashfn_dom vspec.app) { S.length ss = S.length gl }
+  = admit()
+
+let evict_sseq (#vspec:_) (gl: verifiable_log vspec)
+  : ss:sseq (ms_hashfn_dom vspec.app) { S.length ss = S.length gl }
+  = admit()
+
+let appfn_calls
+  (#vspec: verifier_spec)
+  (gl: verifiable_log vspec): sseq (Zeta.AppSimulate.appfn_call_res vspec.app)
+  = admit()
+
+let appfn_calls_within_ep
+  (#vspec: verifier_spec)
+  (ep: epoch)
+  (gl: verifiable_log vspec): sseq (Zeta.AppSimulate.appfn_call_res vspec.app)
+  = admit()
