generic/Zeta.Generic.Global.fsti
@@ -3,9 +3,8 @@ module Zeta.Generic.Global
 open FStar.Seq
 open Zeta.SeqAux
 open Zeta.SSeq
-open Zeta.IdxFn
-open Zeta.SIdxFn
 open Zeta.Interleave
+open Zeta.MultiSet.SSeq
 open Zeta.Time
 open Zeta.MultiSetHashDomain
 open Zeta.GenericVerifier
@@ -31,59 +30,86 @@ let indexss #vspec (gl: vlog vspec) (i: SS.sseq_index gl) =
 let verifiable #vspec (gl: vlog vspec) =
   forall (tid: SA.seq_index gl). {:pattern T.verifiable (thread_log_base gl tid)} T.verifiable (thread_log_base gl tid)
 
-let verifiable_log vspec = gl:vlog vspec {verifiable gl}
+let verifiable_log (vspec: verifier_spec) = gl:vlog vspec {verifiable gl}
 
 val lemma_prefix_verifiable (#vspec:_) (gl: verifiable_log vspec) (l: nat{l <= S.length gl})
   : Lemma (ensures (verifiable (SA.prefix gl l)))
           [SMTPat (SA.prefix gl l)]
 
 let prefix (#vspec:_) (gl: verifiable_log vspec) (l: nat{l <= S.length gl})
-  : gl':verifiable_log vspec {S.length gl' = l}
+  : verifiable_log vspec
   = SA.prefix gl l
 
 let index (#vspec:_) (gl: verifiable_log vspec) (i: SA.seq_index gl)
   : T.verifiable_log vspec
   = thread_log_base gl i
 
-let gso (vspec: verifier_spec) : gen_seq_spec = {
-  seq_t = verifiable_log vspec;
-  length = S.length;
-  prefix
-}
+let clock (#vspec:_) (gl: verifiable_log vspec) (i: sseq_index gl)
+  : timestamp
+  = let tid,j = i in
+    let tl = index gl tid in
+    T.clock tl j
 
-let gen_sseq (vspec:verifier_spec): gen_sseq = {
-  gso = gso vspec;
-  gsi = T.gen_seq vspec;
-  index
-}
+let is_appfn (#vspec:_) (gl: verifiable_log vspec) (i: sseq_index gl)
+  : bool
+  = let t,j = i in
+    let tl = index gl t in
+    T.is_appfn tl j
 
-let idxfn (#vspec:verifier_spec) #b (f: T.idxfn_t vspec b) (gl: verifiable_log vspec) (ii: sseq_index gl)
-  = Zeta.SIdxFn.idxfn #b (gen_sseq vspec) f gl ii
+open Zeta.AppSimulate
 
-let cond_idxfn (#b:_) (#vspec:verifier_spec) (#f: T.idxfn_t vspec bool)
-  = Zeta.SIdxFn.cond_idxfn #b #(gen_sseq vspec) #f
+let to_appfn_call_res (#vspec:_) (gl: verifiable_log vspec) (i: sseq_index gl{is_appfn gl i})
+  : appfn_call_res vspec.app
+  = let t,j = i in
+    let tl = index gl t in
+    T.to_appfn_call_res tl j
 
-let clock #vspec = idxfn (T.clock #vspec)
+let is_blum_add (#vspec:_) (gl: verifiable_log vspec) (i: sseq_index gl)
+  : bool
+  = let t,j = i in
+    let tl = index gl t in
+    T.is_blum_add tl j
+
+let blum_add_elem (#vspec:_) (gl: verifiable_log vspec) (i: sseq_index gl {is_blum_add gl i})
+  : ms_hashfn_dom vspec.app
+  = let t,j = i in
+    let tl = index gl t in
+    T.blum_add_elem tl j
+
+let is_blum_evict (#vspec:_)(gl: verifiable_log vspec) (i: sseq_index gl)
+  : bool
+  = let t,j = i in
+    let tl = index gl t in
+    T.is_blum_evict tl j
+
+let blum_evict_elem (#vspec:_) (gl: verifiable_log vspec) (i: sseq_index gl {is_blum_evict gl i})
+  : ms_hashfn_dom vspec.app
+  = let t,j = i in
+    let tl = index gl t in
+    T.blum_evict_elem tl j
+
+val add_sseq (#vspec:_) (gl: verifiable_log vspec)
+  : ss:sseq (ms_hashfn_dom vspec.app) { S.length ss = S.length gl }
+
+val evict_sseq (#vspec:_) (gl: verifiable_log vspec)
+  : ss:sseq (ms_hashfn_dom vspec.app) { S.length ss = S.length gl }
 
 (* blum add set elements for a given epoch *)
 let add_set
   (#vspec: verifier_spec)
   (ep: epoch)
-  (gl: verifiable_log vspec): mset_ms_hashfn_dom vspec.app
-  = let open Zeta.MultiSet.SSeq in
-    (* filter map specification that filter by AddB? and maps them to blum add elem *)
-    let fm = to_fm (T.is_blum_add_ep ep) (T.blum_add_elem #vspec) in
-    (* get a seq of seq of blum-add-elems and convert them to multiset *)
-    sseq2mset (filter_map (gen_sseq vspec) fm gl)
+  (gl: verifiable_log vspec)
+  : mset_ms_hashfn_dom vspec.app
+  = let as = add_sseq gl in
+    sseq2mset as
 
 (* blum evict set elements for a given epoch *)
 let evict_set
   (#vspec: verifier_spec)
   (ep: epoch)
   (gl: verifiable_log vspec): mset_ms_hashfn_dom vspec.app
-  = let open Zeta.MultiSet.SSeq in
-    let fm = to_fm (T.is_blum_evict_ep ep) (T.blum_evict_elem #vspec) in
-    sseq2mset (filter_map (gen_sseq vspec) fm gl)
+  = let es = evict_sseq gl in
+    sseq2mset es
 
 (* verifiable log property that add- and evict sets are the same *)
 let aems_equal_for_epoch #vspec
@@ -91,32 +117,21 @@ let aems_equal_for_epoch #vspec
   (gl: verifiable_log vspec) =
   add_set ep gl == evict_set ep gl
 
-let aems_equal_for_epoch_prop #vspec
-  (ep: epoch)
-  (gl: verifiable_log vspec)
-  (epmax: epoch) =
-  ep <= epmax ==> aems_equal_for_epoch ep gl
-
 (* add and evict sets are equal for all epochs upto epmax *)
 let aems_equal_upto #vspec (epmax: epoch) (gl: verifiable_log vspec) =
   forall (ep: epoch).
-  {:pattern aems_equal_for_epoch_prop ep gl epmax}
-  aems_equal_for_epoch_prop ep gl epmax
+  ep <= epmax ==> add_set ep gl == evict_set ep gl
 
 (* global log whose add and evict multisets are equal *)
 let ms_verifiable_log #vspec (ep: epoch)
   = gl:verifiable_log vspec{aems_equal_upto ep gl}
 
 (* filter-mapped sequence of sequence app-function-call results *)
-let appfn_calls
+val appfn_calls
   (#vspec: verifier_spec)
   (gl: verifiable_log vspec): sseq (Zeta.AppSimulate.appfn_call_res vspec.app)
-  = let fm = to_fm (T.is_appfn #vspec) (T.to_appfn_call_res #vspec) in
-    filter_map (gen_sseq vspec) fm gl
 
-let appfn_calls_within_ep
+val appfn_calls_within_ep
   (#vspec: verifier_spec)
   (ep: epoch)
   (gl: verifiable_log vspec): sseq (Zeta.AppSimulate.appfn_call_res vspec.app)
-  = let fm = to_fm (T.is_appfn_within_epoch #vspec ep) (T.to_appfn_call_res #vspec) in
-    filter_map (gen_sseq vspec) fm gl
