generic/Zeta.Generic.Interleave.fst
@@ -1,59 +1,10 @@
 module Zeta.Generic.Interleave
 
-
 let lemma_prefix_verifiable (#vspec:_) (n:_) (il:verifiable_log vspec n) (i:nat{i <= S.length il}):
   Lemma (ensures (verifiable (I.prefix il i)))
   = admit()
 
-let idxn_has_prefix_prop (#vspec:_) (#n:nat) (#b:_) (tfn: T.idxfn_t vspec b)
-  : Lemma (ensures (IF.prefix_property #(gen_seq vspec n) (idxfn_base #_ #n #_ tfn)))
-  = admit()
-
-let idxfn_prefix_property (#vspec:_) (#n:_) (#b:_) (tfn: T.idxfn_t vspec b)
-  (il: verifiable_log vspec n) (j:nat{j <= S.length il}) (i: nat{i < j})
-  : Lemma (ensures (idxfn tfn il i == idxfn tfn (prefix il j) i))
-  = admit()
-
-let idxfnil_prefix_property (#vspec:_) (#n:_) (#b:eqtype) (tfn: T.idxfn_t vspec b)
-  (il: verifiable_log vspec n) (j:nat{j <= S.length il}) (i: nat{i < j})
-  : Lemma (ensures (idxfn_il tfn il i == idxfn_il tfn (prefix il j) i))
-  = admit()
-
-let cond_idxfn_has_prefix_prop (#vspec #n #b #f:_) (m: T.cond_idxfn_t b f)
-  : Lemma (ensures (IF.cond_prefix_property #(gen_seq vspec n) #_ #(idxfn f) (cond_idxfn_base m)))
-  = admit()
-
-let lemma_cond_idxfn (#vspec #n:_) (#b: eqtype) (f:_) (m: T.cond_idxfn_t b f)
-  (il: verifiable_log vspec n)
-  : Lemma (ensures (let fm_il = to_fm (idxfn f) (cond_idxfn_il #vspec #n #_ #_ m) in
-                    let ilb = IF.filter_map fm_il il in
-                    let fm_s = to_fm (idxfn f) (cond_idxfn #vspec #n #_ #_ m) in
-                    let sb = IF.filter_map fm_s il in
-                    sb = i_seq ilb))
-  = admit()
-
-let lemma_filter_map (#vspec #n:_) (#b:eqtype) (#f:_) (m: T.cond_idxfn_t b f)
-    (il: verifiable_log vspec n) (i: seq_index il)
-  : Lemma (ensures (let fmil = to_fm (idxfn f) (cond_idxfn_il #vspec #n #_ #_ m) in
-                    let ilb = IF.filter_map fmil il in
-                    let fm = to_fm f m in
-                    let ssb = SF.filter_map (G.gen_sseq vspec) fm (to_glog il) in
-                    ssb = s_seq ilb))
-  = admit()
-
-let lemma_cond_idxfn_interleave (#vspec #n:_) (#b: eqtype) (#f:_) (m: T.cond_idxfn_t b f)
-  (il: verifiable_log vspec n)
-  : Lemma (ensures (let fm_s = to_fm (idxfn f) (cond_idxfn #vspec #n #_ #_ m) in
-                    let sb = IF.filter_map fm_s il in
-                    let fm = to_fm f m in
-                    let ssb = SF.filter_map (G.gen_sseq vspec) fm (to_glog il) in
-                    I.interleave #b sb ssb))
-  = admit()
-
-let thread_state (#vspec: verifier_spec) (#n:_) (tid:nat{tid < n})
-  : IF.seqfn_t (gen_seq vspec n) (v:vspec.vtls_t {vspec.valid v})
-  = admit()
-
+//#push-options "--query_stats --debug Zeta.Generic.Interleave --debug_level SMTQuery"
 let lemma_cur_thread_state_extend (#vspec: verifier_spec) (#n:_)
   (il: verifiable_log vspec n) (i: seq_index il)
   : Lemma (ensures (let st_pre = cur_thread_state_pre il i in
@@ -61,12 +12,21 @@ let lemma_cur_thread_state_extend (#vspec: verifier_spec) (#n:_)
                     st_post == V.verify_step (I.index il i) st_pre))
   = admit()
 
+//#pop-options
 let lemma_non_cur_thread_state_extend (#vspec: verifier_spec) (#n:_) (tid: nat{tid < n})
   (il: verifiable_log vspec n) (i: seq_index il)
   : Lemma (requires (tid <> src il i))
-          (ensures (let st_pre = IF.to_pre_fn (thread_state tid) il i in
-                    let st_post = IF.to_post_fn (thread_state tid) il i in
+          (ensures (let st_pre = thread_state_pre tid il i in
+                    let st_post = thread_state_post tid il i in
                     st_pre == st_post))
+  = admit()
+
+let add_il (#vspec #n:_) (ep: epoch) (il: verifiable_log vspec n)
+  : interleaving (ms_hashfn_dom vspec.app) n
+  = admit()
+
+let evict_il (#vspec #n:_) (ep: epoch) (il: verifiable_log vspec n)
+  : interleaving (ms_hashfn_dom vspec.app) n
   = admit()
 
 let lemma_add_evict_set_identical_glog_aux (#vspec #n:_) (ep: epoch) (il: verifiable_log vspec n)
@@ -77,3 +37,87 @@ let lemma_add_evict_set_identical_glog_aux (#vspec #n:_) (ep: epoch) (il: verifi
 let lemma_add_evict_set_identical_glog (#vspec #n:_) (epmax: epoch) (il: verifiable_log vspec n)
   : Lemma (ensures (aems_equal_upto epmax il <==> G.aems_equal_upto epmax (to_glog il)))
   = admit()
+
+let appfn_calls_il (#vspec: verifier_spec) (#n:_) (il: verifiable_log vspec n)
+  : interleaving (Zeta.AppSimulate.appfn_call_res vspec.app) n
+  = admit()
+
+(*
+let idxfn_base #vspec #n #b (tfn: T.idxfn_t vspec b)
+  (il: verifiable_log vspec n) (i: seq_index il)
+  : b
+  = G.idxfn #vspec tfn (to_glog il) (i2s_map il i)
+
+val idxn_has_prefix_prop (#vspec:_) (#n:nat) (#b:_) (tfn: T.idxfn_t vspec b)
+  : Lemma (ensures (IF.prefix_property #(gen_seq vspec n) (idxfn_base #_ #n #_ tfn)))
+          [SMTPat (idxfn_base #_ #n #_ tfn)]
+
+let idxfn #b #vspec #n (tfn: T.idxfn_t vspec b)
+  : IF.idxfn_t (gen_seq vspec n) _
+  = idxfn_base tfn
+
+let idxfn_il_base #vspec #n (#b:eqtype) (tfn: T.idxfn_t vspec b)
+  (il: verifiable_log vspec n) (i: seq_index il)
+  : elem_src b n
+  = {e = idxfn tfn il i; s = src il i}
+
+let idxfn_il (#b:eqtype) #vspec #n (tfn: T.idxfn_t vspec b)
+  : IF.idxfn_t (gen_seq vspec n) _
+  = idxfn_il_base tfn
+
+(* this should be =() proof but does not work since some pattern matching does not kick-in *)
+val idxfn_prefix_property (#vspec:_) (#n:_) (#b:_) (tfn: T.idxfn_t vspec b)
+  (il: verifiable_log vspec n) (j:nat{j <= S.length il}) (i: nat{i < j})
+  : Lemma (ensures (idxfn tfn il i == idxfn tfn (prefix il j) i))
+          [SMTPat (idxfn tfn (prefix il j) i)]
+
+val idxfnil_prefix_property (#vspec:_) (#n:_) (#b:eqtype) (tfn: T.idxfn_t vspec b)
+  (il: verifiable_log vspec n) (j:nat{j <= S.length il}) (i: nat{i < j})
+  : Lemma (ensures (idxfn_il tfn il i == idxfn_il tfn (prefix il j) i))
+          [SMTPat (idxfn_il tfn (prefix il j) i)]
+
+let cond_idxfn_base #vspec #n #b #f (m: T.cond_idxfn_t b f)
+  (il: verifiable_log vspec n) (i: seq_index il{idxfn f il i})
+  = G.cond_idxfn m (to_glog il) (i2s_map il i)
+
+val cond_idxfn_has_prefix_prop (#vspec #n #b #f:_) (m: T.cond_idxfn_t b f)
+  : Lemma (ensures (IF.cond_prefix_property #(gen_seq vspec n) #_ #(idxfn f) (cond_idxfn_base m)))
+          [SMTPat (cond_idxfn_base #vspec #n #b #f m)]
+
+let cond_idxfn (#vspec #n #b #f:_) (m: T.cond_idxfn_t b f)
+  : IF.cond_idxfn_t b (idxfn f)
+  = cond_idxfn_base #vspec #n m
+
+let cond_idxfn_il_base #vspec #n (#b:eqtype) #f (m: T.cond_idxfn_t b f)
+  (il: verifiable_log vspec n) (i: seq_index il{idxfn f il i})
+  : elem_src b n
+  = {e = cond_idxfn m il i; s = src il i}
+
+let cond_idxfn_il #vspec #n (#b:eqtype) #f (m: T.cond_idxfn_t b f)
+  : IF.cond_idxfn_t (elem_src b n) (idxfn f)
+  = cond_idxfn_il_base #vspec #n #b #f m
+
+val lemma_cond_idxfn (#vspec #n:_) (#b: eqtype) (f:_) (m: T.cond_idxfn_t b f)
+  (il: verifiable_log vspec n)
+  : Lemma (ensures (let fm_il = to_fm (idxfn f) (cond_idxfn_il #vspec #n #_ #_ m) in
+                    let ilb = IF.filter_map fm_il il in
+                    let fm_s = to_fm (idxfn f) (cond_idxfn #vspec #n #_ #_ m) in
+                    let sb = IF.filter_map fm_s il in
+                    sb = i_seq ilb))
+
+val lemma_filter_map (#vspec #n:_) (#b:eqtype) (#f:_) (m: T.cond_idxfn_t b f)
+    (il: verifiable_log vspec n) (i: seq_index il)
+  : Lemma (ensures (let fmil = to_fm (idxfn f) (cond_idxfn_il #vspec #n #_ #_ m) in
+                    let ilb = IF.filter_map fmil il in
+                    let fm = to_fm f m in
+                    let ssb = SF.filter_map (G.gen_sseq vspec) fm (to_glog il) in
+                    ssb = s_seq ilb))
+
+val lemma_cond_idxfn_interleave (#vspec #n:_) (#b: eqtype) (#f:_) (m: T.cond_idxfn_t b f)
+  (il: verifiable_log vspec n)
+  : Lemma (ensures (let fm_s = to_fm (idxfn f) (cond_idxfn #vspec #n #_ #_ m) in
+                    let sb = IF.filter_map fm_s il in
+                    let fm = to_fm f m in
+                    let ssb = SF.filter_map (G.gen_sseq vspec) fm (to_glog il) in
+                    I.interleave #b sb ssb))
+*)
