generic/Zeta.Generic.Interleave.fsti
@@ -3,10 +3,9 @@ module Zeta.Generic.Interleave
 open FStar.Seq
 open Zeta.SeqAux
 open Zeta.Time
-open Zeta.IdxFn
-open Zeta.SIdxFn
 open Zeta.MultiSet
 open Zeta.MultiSetHashDomain
+open Zeta.AppSimulate
 open Zeta.GenericVerifier
 open Zeta.Generic.Thread
 open Zeta.Generic.Global
@@ -18,24 +17,19 @@ module G = Zeta.Generic.Global
 module I = Zeta.Interleave
 module S = FStar.Seq
 module SA = Zeta.SeqAux
-module IF = Zeta.IdxFn
-module SF = Zeta.SIdxFn
 
 let ilog (vspec: verifier_spec) (n:nat) = interleaving (verifier_log_entry vspec) n
 
 (* valid thread ids of an interleaving *)
 let thread_id #vspec #n (il: ilog vspec n) = t:nat{t < n}
 
-(* to sequence of individual thread-level logs *)
-let to_glog #vspec #n (il: ilog vspec n): G.vlog _
-  = I.s_seq il
-
 let seq_index #vspec #n (il: ilog vspec n) = SA.seq_index il
+
 let length #vspec #n (il: ilog vspec n) = S.length il
 
 (* an interleaving is verifiable is the source logs are verifiable *)
 let verifiable #vspec #n (il: ilog vspec n) =
-  G.verifiable (to_glog il)
+  G.verifiable (I.s_seq il)
 
 let verifiable_log vspec n = il:ilog vspec n {verifiable il}
 
@@ -43,111 +37,52 @@ val lemma_prefix_verifiable (#vspec:_) (n:_) (il:verifiable_log vspec n) (i:nat{
   Lemma (ensures (verifiable (I.prefix il i)))
         [SMTPat (I.prefix il i)]
 
+(* to sequence of individual thread-level logs *)
+let to_glog #vspec #n (il: verifiable_log vspec n): G.verifiable_log _
+  = I.s_seq il
+
 let prefix #vspec #n (il: verifiable_log vspec n) (i:nat{i <= S.length il})
-  : il': verifiable_log vspec n{S.length il' = i}
+  : verifiable_log vspec n
   = I.prefix il i
 
-let gen_seq (vspec:verifier_spec) (n:nat) : gen_seq_spec = {
-  IF.seq_t = verifiable_log vspec n;
-  IF.length = S.length;
-  IF.prefix = prefix
-}
-
-let idxfn_base #vspec #n #b (tfn: T.idxfn_t vspec b)
-  (il: verifiable_log vspec n) (i: seq_index il)
-  : b
-  = G.idxfn #vspec tfn (to_glog il) (i2s_map il i)
-
-val idxn_has_prefix_prop (#vspec:_) (#n:nat) (#b:_) (tfn: T.idxfn_t vspec b)
-  : Lemma (ensures (IF.prefix_property #(gen_seq vspec n) (idxfn_base #_ #n #_ tfn)))
-          [SMTPat (idxfn_base #_ #n #_ tfn)]
-
-let idxfn #b #vspec #n (tfn: T.idxfn_t vspec b)
-  : IF.idxfn_t (gen_seq vspec n) _
-  = idxfn_base tfn
-
-let idxfn_il_base #vspec #n (#b:eqtype) (tfn: T.idxfn_t vspec b)
-  (il: verifiable_log vspec n) (i: seq_index il)
-  : elem_src b n
-  = {e = idxfn tfn il i; s = src il i}
-
-let idxfn_il (#b:eqtype) #vspec #n (tfn: T.idxfn_t vspec b)
-  : IF.idxfn_t (gen_seq vspec n) _
-  = idxfn_il_base tfn
-
-(* this should be =() proof but does not work since some pattern matching does not kick-in *)
-val idxfn_prefix_property (#vspec:_) (#n:_) (#b:_) (tfn: T.idxfn_t vspec b)
-  (il: verifiable_log vspec n) (j:nat{j <= S.length il}) (i: nat{i < j})
-  : Lemma (ensures (idxfn tfn il i == idxfn tfn (prefix il j) i))
-          [SMTPat (idxfn tfn (prefix il j) i)]
-
-val idxfnil_prefix_property (#vspec:_) (#n:_) (#b:eqtype) (tfn: T.idxfn_t vspec b)
-  (il: verifiable_log vspec n) (j:nat{j <= S.length il}) (i: nat{i < j})
-  : Lemma (ensures (idxfn_il tfn il i == idxfn_il tfn (prefix il j) i))
-          [SMTPat (idxfn_il tfn (prefix il j) i)]
-
-let cond_idxfn_base #vspec #n #b #f (m: T.cond_idxfn_t b f)
-  (il: verifiable_log vspec n) (i: seq_index il{idxfn f il i})
-  = G.cond_idxfn m (to_glog il) (i2s_map il i)
-
-val cond_idxfn_has_prefix_prop (#vspec #n #b #f:_) (m: T.cond_idxfn_t b f)
-  : Lemma (ensures (IF.cond_prefix_property #(gen_seq vspec n) #_ #(idxfn f) (cond_idxfn_base m)))
-          [SMTPat (cond_idxfn_base #vspec #n #b #f m)]
-
-let cond_idxfn (#vspec #n #b #f:_) (m: T.cond_idxfn_t b f)
-  : IF.cond_idxfn_t b (idxfn f)
-  = cond_idxfn_base #vspec #n m
-
-let cond_idxfn_il_base #vspec #n (#b:eqtype) #f (m: T.cond_idxfn_t b f)
-  (il: verifiable_log vspec n) (i: seq_index il{idxfn f il i})
-  : elem_src b n
-  = {e = cond_idxfn m il i; s = src il i}
-
-let cond_idxfn_il #vspec #n (#b:eqtype) #f (m: T.cond_idxfn_t b f)
-  : IF.cond_idxfn_t (elem_src b n) (idxfn f)
-  = cond_idxfn_il_base #vspec #n #b #f m
-
-val lemma_cond_idxfn (#vspec #n:_) (#b: eqtype) (f:_) (m: T.cond_idxfn_t b f)
-  (il: verifiable_log vspec n)
-  : Lemma (ensures (let fm_il = to_fm (idxfn f) (cond_idxfn_il #vspec #n #_ #_ m) in
-                    let ilb = IF.filter_map fm_il il in
-                    let fm_s = to_fm (idxfn f) (cond_idxfn #vspec #n #_ #_ m) in
-                    let sb = IF.filter_map fm_s il in
-                    sb = i_seq ilb))
-
-val lemma_filter_map (#vspec #n:_) (#b:eqtype) (#f:_) (m: T.cond_idxfn_t b f)
-    (il: verifiable_log vspec n) (i: seq_index il)
-  : Lemma (ensures (let fmil = to_fm (idxfn f) (cond_idxfn_il #vspec #n #_ #_ m) in
-                    let ilb = IF.filter_map fmil il in
-                    let fm = to_fm f m in
-                    let ssb = SF.filter_map (G.gen_sseq vspec) fm (to_glog il) in
-                    ssb = s_seq ilb))
-
-val lemma_cond_idxfn_interleave (#vspec #n:_) (#b: eqtype) (#f:_) (m: T.cond_idxfn_t b f)
-  (il: verifiable_log vspec n)
-  : Lemma (ensures (let fm_s = to_fm (idxfn f) (cond_idxfn #vspec #n #_ #_ m) in
-                    let sb = IF.filter_map fm_s il in
-                    let fm = to_fm f m in
-                    let ssb = SF.filter_map (G.gen_sseq vspec) fm (to_glog il) in
-                    I.interleave #b sb ssb))
-
 (* the clock value at every index *)
-let clock #vspec #n = idxfn #_ #vspec #n (T.clock #vspec)
+let clock (#vspec #n:_) (il: verifiable_log vspec n) (i: seq_index il)
+  : timestamp
+  = let ti = i2s_map il i in
+    G.clock (to_glog il) ti
 
-(* sequence of appfn calls and their results upto epoch ep in the interleaved sequence *)
-let to_appfn_call_res #vspec #n = cond_idxfn #vspec #n #_ #_ (T.to_appfn_call_res #vspec)
+let is_appfn (#vspec #n:_) (il: verifiable_log vspec n) (i: seq_index il)
+  : bool
+  = let ti = i2s_map il i in
+    G.is_appfn (to_glog il) ti
 
-val thread_state (#vspec: verifier_spec) (#n:_) (tid:nat{tid < n})
-  : IF.seqfn_t (gen_seq vspec n) (v:vspec.vtls_t {vspec.valid v})
+let to_appfn_call_res (#vspec #n:_) (il: verifiable_log vspec n) (i: seq_index il{is_appfn il i})
+  : appfn_call_res vspec.app
+  = let ti = i2s_map il i in
+    G.to_appfn_call_res (to_glog il) ti
+
+let thread_state (#vspec: verifier_spec) (#n:_) (tid:nat{tid < n}) (il: verifiable_log vspec n)
+  = let gl = to_glog il in
+    let tl = G.index gl tid in
+    T.state tl
+
+let thread_state_pre (#vspec #n:_) (tid:nat{tid < n})
+  (il: verifiable_log vspec n) (i: seq_index il)
+  = let il' = I.prefix il i in
+    thread_state tid il'
+
+let thread_state_post (#vspec #n:_) (tid:nat{tid < n})
+  (il: verifiable_log vspec n) (i: seq_index il)
+  = let il' = I.prefix il (i+1) in
+    thread_state tid il'
 
 let cur_thread_state_pre (#vspec: verifier_spec) (#n:_) (il: verifiable_log vspec n) (i: seq_index il)
-  = let s = src il i in
-    IF.to_pre_fn (thread_state s) il i
+  = let t = src il i in
+    thread_state_pre t il i
 
-let cur_thread_state_post (#vspec: verifier_spec) (#n:_)
-  (il: verifiable_log vspec n) (i: seq_index il)
-  = let s = src il i in
-    IF.to_post_fn (thread_state s) il i
+let cur_thread_state_post (#vspec: verifier_spec) (#n:_) (il: verifiable_log vspec n) (i: seq_index il)
+  = let t = src il i in
+    thread_state_post t il i
 
 val lemma_cur_thread_state_extend (#vspec: verifier_spec) (#n:_)
   (il: verifiable_log vspec n) (i: seq_index il)
@@ -158,40 +93,61 @@ val lemma_cur_thread_state_extend (#vspec: verifier_spec) (#n:_)
 val lemma_non_cur_thread_state_extend (#vspec: verifier_spec) (#n:_) (tid: nat{tid < n})
   (il: verifiable_log vspec n) (i: seq_index il)
   : Lemma (requires (tid <> src il i))
-          (ensures (let st_pre = IF.to_pre_fn (thread_state tid) il i in
-                    let st_post = IF.to_post_fn (thread_state tid) il i in
+          (ensures (let st_pre = thread_state_pre tid il i in
+                    let st_post = thread_state_post tid il i in
                     st_pre == st_post))
 
-let blum_add_elem #vspec #n = cond_idxfn #_ #n #_ #_ (T.blum_add_elem #vspec)
+let is_blum_add (#vspec #n:_) (il: verifiable_log vspec n) (i: seq_index il)
+  : bool
+  = let ti = i2s_map il i in
+    G.is_blum_add (to_glog il) ti
 
-let blum_evict_elem #vspec #n = cond_idxfn #_ #n #_ #_ (T.blum_evict_elem #vspec)
+let blum_add_elem #vspec #n (il: verifiable_log vspec n) (i: seq_index il{is_blum_add il i})
+  : ms_hashfn_dom vspec.app
+  = let ti = i2s_map il i in
+    G.blum_add_elem (to_glog il) ti
+
+let is_blum_evict  (#vspec #n:_) (il: verifiable_log vspec n) (i: seq_index il)
+  : bool
+  = let ti = i2s_map il i in
+    G.is_blum_evict (to_glog il) ti
+
+let blum_evict_elem #vspec #n (il: verifiable_log vspec n) (i: seq_index il{is_blum_evict il i})
+  : ms_hashfn_dom vspec.app
+  = let ti = i2s_map il i in
+    G.blum_evict_elem (to_glog il) ti
+
+val add_il (#vspec #n:_) (ep: epoch) (il: verifiable_log vspec n)
+  : interleaving (ms_hashfn_dom vspec.app) n
+
+let add_seq (#vspec #n:_) (ep: epoch) (il: verifiable_log vspec n)
+  : S.seq (ms_hashfn_dom vspec.app)
+  = i_seq (add_il ep il)
 
 let add_set #vspec #n (ep: epoch) (il: verifiable_log vspec n)
   : mset_ms_hashfn_dom vspec.app
-  = let fm = IF.to_fm (idxfn (T.is_blum_add_ep ep)) blum_add_elem in
-    seq2mset (IF.filter_map fm il)
+  = seq2mset (add_seq ep il)
+
+val evict_il (#vspec #n:_) (ep: epoch) (il: verifiable_log vspec n)
+  : interleaving (ms_hashfn_dom vspec.app) n
+
+let evict_seq (#vspec #n:_) (ep: epoch) (il: verifiable_log vspec n)
+  : S.seq (ms_hashfn_dom vspec.app)
+  = i_seq (evict_il ep il)
 
 let evict_set #vspec #n (ep: epoch) (il: verifiable_log vspec n)
   : mset_ms_hashfn_dom vspec.app
-  = let fm = IF.to_fm (idxfn (T.is_blum_evict_ep ep)) blum_evict_elem in
-    seq2mset (IF.filter_map fm il)
-
-let aems_equal_for_epoch_prop #vspec #n (ep epmax: epoch) (il: verifiable_log vspec n)
-  = ep <= epmax ==> add_set ep il == evict_set ep il
+  = seq2mset (evict_seq ep il)
 
 let aems_equal_upto #vspec #n (epmax: epoch) (il: verifiable_log vspec n)
-  = forall (ep: epoch). {:pattern aems_equal_for_epoch_prop ep epmax il} aems_equal_for_epoch_prop ep epmax il
+  = forall (ep: epoch). ep <= epmax ==> add_set ep il == evict_set ep il
 
 val lemma_add_evict_set_identical_glog (#vspec #n:_) (epmax: epoch) (il: verifiable_log vspec n)
   : Lemma (ensures (aems_equal_upto epmax il <==> G.aems_equal_upto epmax (to_glog il)))
 
+val appfn_calls_il (#vspec: verifier_spec) (#n:_) (il: verifiable_log vspec n)
+  : interleaving (Zeta.AppSimulate.appfn_call_res vspec.app) n
+
 let appfn_calls (#vspec: verifier_spec) (#n:_) (il: verifiable_log vspec n)
   : seq (Zeta.AppSimulate.appfn_call_res vspec.app)
-  = let fm = IF.to_fm (idxfn T.is_appfn) to_appfn_call_res in
-    IF.filter_map fm il
-
-let appfn_calls_il (#vspec: verifier_spec) (#n:_) (il: verifiable_log vspec n)
-  : interleaving (Zeta.AppSimulate.appfn_call_res vspec.app) n
-  = let ifn = cond_idxfn_il #vspec #n #_ #_ (T.to_appfn_call_res #vspec)  in
-    let fm = to_fm (idxfn T.is_appfn) ifn in
-    IF.filter_map fm il
+  = i_seq (appfn_calls_il il)
