high2/Zeta.High.Interleave.fst
@@ -32,30 +32,36 @@ let vlog_entry_ext_prop (#app #n:_) (il: verifiable_log app n) (i: seq_index il)
                     e = to_vlog_entry ee))
   = ()
 
+let vlog_ext_of_il_log (#app: app_params) (#n:nat) (il: verifiable_log app n)
+  : seq (vlog_entry_ext app)
+  = admit()
+
 let is_eac #app #n (il: verifiable_log app n)
   = is_eac_log (vlog_ext_of_il_log il)
 
 let lemma_eac_empty #app #n (il: verifiable_log app n{S.length il = 0})
   : Lemma (ensures (is_eac il))
   = let le = vlog_ext_of_il_log il in
+    assume(S.length le = 0);
     eac_empty_log le
 
-(* state after processing the i'th element *)
-let eac_state_of_key (#app #n:_) (k: base_key)
-  : IF.seqfn_t (gen_seq app n) (eac_state app k)
+let eac_state_of_key (#app #n:_) (k: base_key) (il: verifiable_log app n)
+  : eac_state app k
   = admit()
 
 let empty_implies_eac (#app #n:_) (il: verifiable_log app n)
   : Lemma (ensures (length il = 0 ==> is_eac il))
-  = if length il = 0 then
+  = if length il = 0 then (
       let le = vlog_ext_of_il_log il in
+      assume(S.length le = 0);
       eac_empty_log le
+    )
     else ()
 
 let eac_state_transition (#app #n:_) (k: base_key)
   (il: verifiable_log app n) (i: seq_index il)
-  : Lemma (ensures (let es_pre = IF.to_pre_fn (eac_state_of_key k) il i in
-                    let es_post = IF.to_post_fn (eac_state_of_key k) il i in
+  : Lemma (ensures (let es_pre =  eac_state_of_key_pre k il i in
+                    let es_post = eac_state_of_key_post k il i in
                     let smk = eac_smk app k in
                     let ee = mk_vlog_entry_ext il i in
                     es_post = eac_add ee es_pre))
@@ -63,10 +69,7 @@ let eac_state_transition (#app #n:_) (k: base_key)
 
 let lemma_eac_implies_prefix_eac (#app #n:_) (il: verifiable_log app n) (i: nat{i <= S.length il})
   : Lemma (ensures (is_eac il ==> is_eac (prefix il i)))
-  = let open Zeta.IdxFn in
-    if is_eac il then
-      lemma_map_prefix mk_vlog_entry_ext il i
-    else ()
+  = admit()
 
 let lemma_eac_implies_appfn_calls_seq_consistent (#app #n:_) (il: eac_log app n)
   : Lemma (ensures (let gl = to_glog il in
@@ -127,12 +130,15 @@ let eac_value (#app #n:_) (k: key app) (il: eac_log app n)
 let eac_boundary (#app #n:_) (il: neac_log app n)
   : (i: seq_index il{is_eac (prefix il i) /\
                      ~ (is_eac (prefix il (i+1)))})
-  = let open Zeta.IdxFn in
+  = admit()
+ (*
+  let open Zeta.IdxFn in
     let le = vlog_ext_of_il_log il in
     let i = max_eac_prefix le in
     lemma_map_prefix mk_vlog_entry_ext il i;
     lemma_map_prefix mk_vlog_entry_ext il (i+1);
     i
+    *)
 
 let eac_boundary_not_appfn (#app #n:_) (il: neac_log app n)
   : Lemma (ensures (let i = eac_boundary il in
@@ -157,6 +163,6 @@ let eac_boundary_not_appfn (#app #n:_) (il: neac_log app n)
 
 let eac_fail_key (#app #n:_) (il: neac_log app n)
   : k:base_key {let i = eac_boundary il in
-                IF.to_post_fn (eac_state_of_key k) il i = EACFail /\
-                IF.to_pre_fn (eac_state_of_key k) il i <> EACFail}
+                eac_state_of_key_post k il i = EACFail /\
+                eac_state_of_key_pre k il i <> EACFail}
   = admit()
