high2/Zeta.High.Global.fsti
@@ -10,7 +10,5 @@ let vlog (app:app_params) = Zeta.Generic.Global.vlog (high_verifier_spec app)
 let verifiable_log (app:_)
   = Zeta.Generic.Global.verifiable_log (high_verifier_spec app)
 
-let gen_sseq (app: app_params) = Zeta.Generic.Global.gen_sseq (high_verifier_spec app)
-
 let ms_verifiable_log (app: app_params) (ep: epoch)
   = Zeta.Generic.Global.ms_verifiable_log #(high_verifier_spec app) ep
